proof/crefine/ARM/TcbAcc_C.thy
@@ -94,13 +94,14 @@ lemma getRegister_ccorres [corres]:
        apply (drule (1) obj_at_cslift_tcb)
        apply (clarsimp simp: typ_heap_simps register_from_H_less)
        apply (clarsimp simp: getRegister_def typ_heap_simps)
-       apply (rule_tac x = "((atcbContextGet o tcbArch) ko reg, \<sigma>)" in bexI [rotated])
+       apply (rule_tac x = "((user_regs o atcbContextGet o tcbArch) ko reg, \<sigma>)" in bexI[rotated])
         apply (simp add: in_monad' asUser_def select_f_def split_def)
         apply (subst arg_cong2 [where f = "(\<in>)"])
           defer
           apply (rule refl)
          apply (erule threadSet_eq)
-        apply (clarsimp simp: ctcb_relation_def ccontext_relation_def carch_tcb_relation_def)
+        apply (clarsimp simp: ctcb_relation_def ccontext_relation_def cregs_relation_def
+                              carch_tcb_relation_def)
        apply (wp threadGet_obj_at2)+
    apply simp
   apply simp
