proof/crefine/ARM_HYP/Fastpath_Equiv.thy
@@ -244,7 +244,7 @@ lemma ctes_of_Some_cte_wp_at:
   by (clarsimp simp: cte_wp_at_ctes_of)
 
 lemma user_getreg_wp:
-  "\<lbrace>\<lambda>s. tcb_at' t s \<and> (\<forall>rv. obj_at' (\<lambda>tcb. (atcbContextGet o tcbArch) tcb r = rv) t s \<longrightarrow> Q rv s)\<rbrace>
+  "\<lbrace>\<lambda>s. tcb_at' t s \<and> (\<forall>rv. obj_at' (\<lambda>tcb. (user_regs o atcbContextGet o tcbArch) tcb r = rv) t s \<longrightarrow> Q rv s)\<rbrace>
       asUser t (getRegister r) \<lbrace>Q\<rbrace>"
   apply (rule_tac Q="\<lambda>rv s. \<exists>rv'. rv' = rv \<and> Q rv' s" in hoare_post_imp)
    apply simp
@@ -733,7 +733,8 @@ lemma fastpath_callKernel_SysCall_corres:
                      apply (rule monadic_rewrite_weaken_flags[where F=False and E=True], simp)
                      apply (rule isolate_thread_actions_rewrite_bind
                                  fastpath_isolate_rewrites fastpath_isolatables
-                                 bool.simps setRegister_simple
+                                 bool.simps setRegister_simple_modify_registers
+                                 zipWithM_setRegister_simple_modify_registers
                                  threadGet_vcpu_isolatable[THEN thread_actions_isolatableD, simplified o_def]
                                  threadGet_vcpu_isolatable[simplified o_def]
                                  vcpuSwitch_isolatable[THEN thread_actions_isolatableD] vcpuSwitch_isolatable
@@ -741,7 +742,6 @@ lemma fastpath_callKernel_SysCall_corres:
                                  doMachineOp_isolatable[THEN thread_actions_isolatableD] doMachineOp_isolatable
                                  kernelExitAssertions_isolatable[THEN thread_actions_isolatableD]
                                  kernelExitAssertions_isolatable
-                                 zipWithM_setRegister_simple
                                  thread_actions_isolatable_bind
                               | assumption
                               | wp assert_inv)+
@@ -1648,8 +1648,8 @@ lemma fastpath_callKernel_SysReplyRecv_corres:
                       apply (rule monadic_rewrite_weaken_flags[where F=False and E=True], simp)
                       apply (rule isolate_thread_actions_rewrite_bind
                                   fastpath_isolate_rewrites fastpath_isolatables
-                                  bool.simps setRegister_simple
-                                  zipWithM_setRegister_simple
+                                  bool.simps setRegister_simple_modify_registers
+                                  zipWithM_setRegister_simple_modify_registers
                                   thread_actions_isolatable_bind
                                   thread_actions_isolatableD[OF setCTE_isolatable]
                                   setCTE_isolatable
