proof/drefine/StateTranslation_D.thy
@@ -755,7 +755,8 @@ where
 definition
   get_tcb_message_info :: "tcb \<Rightarrow> Structures_A.message_info"
 where
-  "get_tcb_message_info t \<equiv> data_to_message_info ((arch_tcb_context_get (tcb_arch t)) msg_info_register)"
+  "get_tcb_message_info t \<equiv>
+     data_to_message_info ((user_regs (arch_tcb_context_get (tcb_arch t))) msg_info_register)"
 
 definition
   get_tcb_mrs :: "machine_state \<Rightarrow> tcb \<Rightarrow> word32 list"
@@ -763,7 +764,7 @@ where
   "get_tcb_mrs ms tcb \<equiv>
     let
       info = get_tcb_message_info tcb;
-      cpu_mrs = map (arch_tcb_context_get (tcb_arch tcb)) msg_registers;
+      cpu_mrs = map (user_regs (arch_tcb_context_get (tcb_arch tcb))) msg_registers;
       mem_mrs = get_ipc_buffer_words ms tcb [length msg_registers + 1 ..< Suc msg_max_length]
     in
       (take (unat (mi_length info)) (cpu_mrs @ mem_mrs))"
@@ -782,7 +783,7 @@ where
                      (invocation_type (mi_label mi))
                      (get_tcb_mrs ms tcb)),
     cdl_intent_error = guess_error (mi_label mi),
-    cdl_intent_cap = arch_tcb_context_get (tcb_arch tcb) cap_register,
+    cdl_intent_cap = user_regs (arch_tcb_context_get (tcb_arch tcb)) cap_register,
     cdl_intent_extras = get_ipc_buffer_words ms tcb [buffer_cptr_index ..< buffer_cptr_index + (unat (mi_extra_caps mi))],
     cdl_intent_recv_slot = case (get_ipc_buffer_words ms tcb [offset ..< offset + 3]) of
                                 [croot, index, depth] \<Rightarrow> Some (croot, index, unat depth)
